spec_sub

SP1Chips/SubChip.lean
@@ -16,7 +16,7 @@ variable
   (cstrs : (constraints Main).allHold)
   (h_is_real : Main[32] = 1)
 
-def spec_add (rs2 rs1 rd : regidx) : SailM Unit := do
+def spec_sub (rs2 rs1 rd : regidx) : SailM Unit := do
   Sail.writeReg Register.nextPC ((← Sail.readReg Register.PC) + 4#64)
   _ ← execute (.RTYPE (rs2, rs1, rd, rop.SUB))
   pure ()
@@ -78,7 +78,7 @@ theorem correct_add
   let op_c := sp1_op_c Main cstrs h_is_real
   let op_b := sp1_op_b Main cstrs h_is_real
   let op_a := sp1_op_a Main cstrs h_is_real
-  (spec_add (.Regidx op_c) (.Regidx op_b) (.Regidx op_a)).run s = (sp1_add Main cstrs h_is_real).run s
+  (spec_sub (.Regidx op_c) (.Regidx op_b) (.Regidx op_a)).run s = (sp1_add Main cstrs h_is_real).run s
   := by
     -- Obtain and simplify state and pure constraints
     simp [SP1ConstraintList.initialState, constraints, SP1Constraint.toStateProp, List.Forall, SubOperation.constraints, CPUState.constraints, RTypeReader.constraints, h_is_real] at state_cstrs
@@ -95,7 +95,7 @@ theorem correct_add
     simp at *
 
     -- Now the monadic manipulation
-    simp [spec_add, sp1_add, execute, execute_RTYPE']
+    simp [spec_sub, sp1_add, execute, execute_RTYPE']
     rw [run_readReg, read_pc]
     simp [sp1_op_b, read_op_b (by omega)]
     simp [sp1_op_c, read_op_c (by omega)]
